move [Addr_as_OT] into Prog.v

src/MemLog.v
@@ -19,40 +19,6 @@ Require Import Eqdep_dec.
 Require Import GenSep.
 Require Import WordAuto.
 
-(* XXX parameterize by length and stick in Word.v *)
-Module Addr_as_OT <: UsualOrderedType.
-  Definition t := addr.
-  Definition eq := @eq t.
-  Definition eq_refl := @eq_refl t.
-  Definition eq_sym := @eq_sym t.
-  Definition eq_trans := @eq_trans t.
-  Definition lt := @wlt addrlen.
-
-  Lemma lt_trans: forall x y z : t, lt x y -> lt y z -> lt x z.
-  Proof.
-    unfold lt; intros.
-    apply wlt_lt in H; apply wlt_lt in H0.
-    apply lt_wlt.
-    omega.
-  Qed.
-
-  Lemma lt_not_eq : forall x y : t, lt x y -> ~ eq x y.
-  Proof.
-    unfold lt, eq; intros.
-    apply wlt_lt in H.
-    intro He; subst; omega.
-  Qed.
-
-  Definition compare x y : Compare lt eq x y.
-    unfold lt, eq.
-    destruct (wlt_dec x y); [ apply LT; auto | ].
-    destruct (weq x y); [ apply EQ; auto | ].
-    apply GT. apply le_neq_lt; auto.
-  Defined.
-
-  Definition eq_dec := @weq addrlen.
-End Addr_as_OT.
-
 Module Map := FMapList.Make(Addr_as_OT).
 
 Import ListNotations.
